trying alt approach

Stlc.v
@@ -1,6 +1,82 @@
 Require Import Lambda.Util Coq.Program.Equality.
 Require Import FunctionalExtensionality.
 
+Section NthError.
+  Context {A : Type}.
+  
+  Lemma nth_error_nil : forall n, nth_error (@nil A) n = None.
+  Proof. intros []; reflexivity. Qed.
+
+  Hint Rewrite nth_error_nil : core.
+
+  Lemma nth_error_length : forall (l : list A) n a,
+      nth_error l n = Some a -> n < length l.
+  Proof.
+    intro l; induction l as [| h t IHt];
+      intros [| n]; simpl; intros a H;
+        autorewrite with core in *; try discriminate; try lia.
+    apply IHt in H. lia.
+  Qed.
+
+  Lemma nth_error_app_plus : forall (l l' : list A) n,
+      nth_error (l ++ l') (length l + n) = nth_error l' n.
+  Proof.
+    intros l l' n.
+    rewrite nth_error_app2 by lia.
+    f_equal; lia.
+  Qed.
+
+  Lemma nth_map : forall B (f : A -> B) l n a b,
+      n < length l ->
+      nth n (map f l) b = f (nth n l a).
+  Proof.
+    induction l as [| h t IHt];
+      intros [| n] a b; simpl; intros; try lia; auto.
+    apply IHt; lia.
+  Qed.
+
+  Lemma length_nth_error : forall (l : list A) n,
+      n < length l -> exists a, nth_error l n = Some a.
+  Proof.
+    intro l; induction l as [| h t IHt];
+      intros [| n] H; simpl in *; try lia; eauto.
+    apply IHt. lia.
+  Qed.
+End NthError.
+
+Section Forall2.
+  Variables A B : Type.
+  Variable R : A -> B -> Prop.
+  
+  Lemma Forall2_length : forall a b,
+    Forall2 R a b -> length a = length b.
+  Proof.
+    intros a b H; induction H; simpl; auto.
+  Qed.
+  
+  Lemma Forall2_impl : forall (Q : A -> B -> Prop) a b,
+      (forall a b, R a b -> Q a b) ->
+      Forall2 R a b -> Forall2 Q a b.
+  Proof.
+    intros Q a b H HP;
+      induction HP; auto.
+  Qed.
+
+  Lemma Forall2_nth_error : forall la lb,
+      Forall2 R la lb ->
+      forall n a b, nth_error la n = Some a ->
+               nth_error lb n = Some b ->
+               R a b.
+  Proof.
+    intros la lb HR; induction HR;
+      intros [| n] a b Hntha Hnthb;
+      simpl in *; try discriminate.
+    - inv Hntha; inv Hnthb. assumption.
+    - pose proof IHHR _ _ _ Hntha Hnthb.
+      assumption.
+  Qed.
+End Forall2.
+
 (** * De Bruijn Syntax *)
 
 Inductive type : Set :=
@@ -23,7 +99,8 @@ Inductive expr : Set :=
 Declare Scope expr_scope.
 Delimit Scope expr_scope with expr.
 Notation "'λ' t '⇒' e" := (Lam t e) (at level 10) : expr_scope.
-Notation "e1 ⋅ e2" := (App e1 e2) (at level 8, left associativity) : expr_scope.
+Notation "e1 ⋅ e2"
+  := (App e1 e2) (at level 8, left associativity) : expr_scope.
 Notation "! n" := (Var n) (at level 0) : expr_scope.
 Open Scope expr_scope.
 
@@ -35,7 +112,7 @@ Example t1 : type := (⊥ → ⊥) → ⊥ → ⊥.
 
 Reserved Notation "Γ '⊢' e '∈' τ" (at level 40).
 
-Inductive check (Γ : list type) : expr -> type -> Prop :=
+Inductive typing (Γ : list type) : expr -> type -> Prop :=
 | chk_var n τ :
     nth_error Γ n = Some τ ->
     Γ ⊢ !n ∈ τ
@@ -46,7 +123,7 @@ Inductive check (Γ : list type) : expr -> type -> Prop :=
     Γ ⊢ e1 ∈ τ → τ' ->
     Γ ⊢ e2 ∈ τ ->
     Γ ⊢ e1 ⋅ e2 ∈ τ'
-where "Γ '⊢' e '∈' τ" := (check Γ e τ).
+where "Γ '⊢' e '∈' τ" := (typing Γ e τ).
 (**[]*)
 
 Theorem type_unique : forall Γ e τ1 τ2,
@@ -61,15 +138,26 @@ Proof.
     inv IH1; reflexivity.
 Qed.
 
+Section TypingLemmas.
+  Local Hint Constructors typing : core.
+  Local Hint Resolve nth_error_app1 : core.
+  Local Hint Resolve nth_error_length : core.
+
+  Lemma typing_prefix G e t :
+      G ⊢ e ∈ t -> forall g, (G ++ g) ⊢ e ∈ t.
+  Proof.
+    intros H; induction H;
+      intros g; eauto.
+    constructor. rewrite nth_error_app1; eauto.
+  Qed.
+End TypingLemmas.
+
 (** * Dynamic Semantics *)
 
 (** Shifts free variables above a cutoff [c] up by [i]. *)
 Fixpoint shift (c i : nat) (e : expr) : expr :=
   match e with
-  | !n =>  ! match lt_dec n c with
-            | left _ => n
-            | right _ => n + i
-            end
+  | !n => ! if le_lt_dec c n then n + i else n
   | λ τ ⇒ e => λ τ ⇒ (shift (S c) i e)
   | e1 ⋅ e2 => (shift c i e1) ⋅ (shift c i e2)
   end.
@@ -83,336 +171,66 @@ Section ShiftLemmas.
   Lemma shift0 : forall e k, shift k 0 e = e.
   Proof. induction e; destroy_arith. Qed.
 
-  Lemma simpl_shift : forall e n p k i,
-      i <= k + n -> k <= i ->
-      shift i p (shift k n e) = shift k (p + n) e.
+  Lemma shift_add : forall e d d' c c',
+    c <= c' <= c + d -> shift c' d' (shift c d e) = shift c (d' + d) e.
   Proof.
-    induction e; destroy_arith.
-    f_equal; apply IHe; lia.
+    induction e as [n | t e IHe | e1 IHe1 e2 IHe2];
+      intros; simpl.
+    - destroy_arith.
+    - rewrite IHe by lia. reflexivity.
+    - f_equal; auto.
   Qed.
 
-  Local Hint Extern 0 => rewrite simpl_shift by lia; reflexivity : core.
-
-  Lemma permute_shift : forall e n k p i,
-      i <= k -> shift i p (shift k n e) = shift (p + k) n (shift i p e).
+  Lemma shift_shift_distr : forall e d c d' c',
+      c' <= c -> shift c' d' (shift c d e) = shift (d' + c) d (shift c' d' e).
   Proof.
-    induction e; destroy_arith.
-    f_equal; rewrite IHe; f_equal; lia.
+    induction e as [n | t e IHe | e1 IHe1 e2 IHe2];
+      intros; simpl; f_equal; auto.
+    - destroy_arith.
+    - rewrite IHe by lia. f_equal; lia.
   Qed.
 
-  Local Hint Extern 0 => rewrite permute_shift by lia; reflexivity : core.
-End ShiftLemmas.
-
-(** Substitution [e{esub/i}].
-    [5 6 7 (esub/6) = 4 (shift 0 6 esub) 7]
- *)
-Fixpoint sub (i : nat) (esub e : expr) : expr :=
-  match e with
-  | !n => match lt_eq_lt_dec i n with
-         | inleft (left _) => ! (pred n)
-         | inleft (right _) => shift 0 i esub
-         | inright _ => !n
-         end
-  | λ τ ⇒ e => λ τ ⇒ (sub (S i) esub e)
-  | e1 ⋅ e2 => (sub i esub e1) ⋅ (sub i esub e2)
-  end.
-(**[]*)
-
-Section SubShiftLemmas.
-  Local Hint Extern 0 => rewrite simpl_shift by lia; reflexivity : core.
-  Local Hint Extern 0 => rewrite permute_shift by lia; reflexivity : core.
-
-  Lemma simpl_sub : forall M N n p k,
-    p <= n + k -> k <= p ->
-    sub p N (shift k (S n) M) = shift k n M.
-  Proof.
-    induction M; destroy_arith.
-    f_equal; apply IHM; lia.
-  Qed.
-
-  Local Hint Extern 0 => rewrite simpl_sub by lia; reflexivity : core.
-
-  Lemma commute_shift_sub : forall M N n p k,
-      k <= p ->
-      shift k n (sub p N M) = sub (n + p) N (shift k n M).
-  Proof.
-    induction M; destroy_arith.
-    f_equal; rewrite IHM; f_equal; lia.
-  Qed.
-
-  Local Hint Extern 0 => rewrite commute_shift_sub by lia; reflexivity : core.
+  Local Hint Constructors typing : core.
   
-  Lemma distr_shift_sub : forall M N n p k,
-      shift (p + k) n (sub p N M) = sub p (shift k n N) (shift (S (p + k)) n M).
-  Proof.
-    induction M; destroy_arith.
-    f_equal; rewrite <- IHM; f_equal; lia.
-  Qed.
-
-  Lemma distr_sub : forall M N P n p,
-      sub (p + n) P (sub p N M) =
-      sub p (sub n P N) (sub (S (p + n)) P M).
-  Proof.
-    induction M; destroy_arith.
-    f_equal; rewrite <- IHM; f_equal; lia.
-  Qed.
-End SubShiftLemmas.
-
-(** Beta-reduction [(λx.e1) e2 -> e1{e2/x}]. *)
-Definition beta_reduce (e1 e2 : expr) : expr := sub 0 e2 e1.
-(**[]*)
-
-Lemma distr_shift_beta : forall M N n k,
-    shift k n (beta_reduce M N) = beta_reduce (shift (S k) n M) (shift k n N).
-Proof.
-  intros; unfold beta_reduce.
-  replace k with (0 + k) at 1 by lia.
-  replace k with (0 + k) at 3 by lia.
-  apply distr_shift_sub.
-Qed.
-
-Lemma distr_sub_beta : forall M N P n,
-    sub n P (beta_reduce M N) =
-    beta_reduce (sub (S n) P M) (sub n P N).
-Proof.
-  intros; unfold beta_reduce.
-  replace n with (0 + n) at 1 by lia.
-  replace n with (0 + n) at 3 by lia.
-  apply distr_sub.
-Qed.
-
-(** Call-by-value Reduction. *)
-
-Inductive is_lam : expr -> Prop :=
-| is_lam_intro t e : is_lam (λ t ⇒ e).
-
-Inductive stuck : expr -> Prop :=
-| stuck_var n :
-    stuck !n
-| stuck_lam t e :
-    stuck (λ t ⇒ e)
-| stuck_app e1 e2 :
-    ~ is_lam e1 ->
-    stuck e1 -> stuck e2 -> stuck (e1 ⋅ e2).
-(**[]*)
-
-Reserved Notation "e1 '-->' e2" (at level 40).
-
-Inductive step : expr -> expr -> Prop :=
-| step_beta τ e1 e2 :
-    stuck e2 ->
-    (λ τ ⇒ e1) ⋅ e2 -->  beta_reduce e1 e2
-| step_app_r e1 e2 e2' :
-    stuck e1 ->
-    e2 -->  e2' ->
-    e1 ⋅ e2 -->  e1 ⋅ e2'
-| step_app_l e1 e1' e2 :
-    e1 -->  e1' ->
-    e1 ⋅ e2 -->  e1' ⋅ e2
-where "e1 '-->' e2" := (step e1 e2).
-(**[]*)
-
-Ltac inv_step_bad :=
-  match goal with
-  | H: !_ -->  _ |- _ => inv H
-  | H: λ _ ⇒ _ -->  _ |- _ => inv H
-  end.
-
-Section NormalForm.
-  Local Hint Constructors stuck : core.
-
-  Ltac contra_step :=
-    match goal with
-    | H: ?e -->  _, IH : (forall _, ~ ?e -->  _)
-      |- _ => apply IH in H; contradiction
-    end.
-
-  Local Hint Extern 0 => contra_step : core.
-  Local Hint Extern 0 => inv_step_bad : core.
-  Local Hint Constructors is_lam : core.
-
-  Lemma step_nstuck : forall e e',
-      e -->  e' -> ~ stuck e.
-  Proof.
-    intros ? ? Hs Hstk;
-      induction Hs; inv Hstk; eauto.
-  Qed.
-  
-  Lemma stuck_step : forall e e',
-      stuck e -> ~ e -->  e'.
-  Proof.
-    intros ? e' Hv;
-      generalize dependent e';
-      induction Hv; intros ? He; inv He; eauto.
-  Qed.
-End NormalForm.
-
-Ltac stuck_step_contra :=
-  match goal with
-  | Hnf: stuck ?e, He: ?e -->  _
-    |- _ => pose proof stuck_step _ _ Hnf He;
-          contradiction
-  end.
-(**[]*)
-
-Section Determinism.
-  Local Hint Constructors is_lam : core.
-  Local Hint Constructors stuck : core.
-  Local Hint Extern 0 => inv_step_bad : core.
-  Local Hint Extern 0 => stuck_step_contra : core.
-
-  Theorem step_deterministic : deterministic step.
-  Proof. ind_det; f_equal; eauto 2. Qed.
-End Determinism.
-
-Section CanonicalForms.
-  Lemma nth_error_nil : forall A n,
-    @nth_error A [] n = None.
-  Proof. intros ? []; reflexivity. Qed.
-
-  Hint Rewrite nth_error_nil : core.
-  Local Hint Constructors stuck : core.
-  Local Hint Constructors is_lam : core.
-
-  Lemma is_lam_exm : forall e, is_lam e \/ ~ is_lam e.
-  Proof.
-    intros []; intuition;
-      right; intros H; inv H; contradiction.
-  Qed.
-
-  Local Hint Resolve is_lam_exm : core.
-
-  Lemma stuck_exm : forall e,
-      stuck e \/ ~ stuck e.
+  Lemma typing_shift : forall e G g g' t,
+      (G ++ g) ⊢ e ∈ t ->
+      (G ++ g' ++ g) ⊢ (shift (length G) (length g') e) ∈ t.
   Proof.
     intro e;
-      induction e as
-        [ n
-        | t e ?
-        | e1 [IHe1 | IHe1] e2 [IHe2 | IHe2]];
-      intuition;
-      try (right; intros H; inv H; contradiction).
-    destruct (is_lam_exm e1); intuition.
-    right; intros H'; inv H'; contradiction.
-  Qed.
-  
-  Lemma canonical_forms_lambda : forall e τ τ',
-    stuck e -> [] ⊢ e ∈ τ → τ' -> exists e', e = λ τ ⇒ e'.
-  Proof.
-    intros ? t t' Hnf;
-      generalize dependent t';
-      generalize dependent t;
-      induction Hnf; intros ? ? Ht; inv Ht;
-        autorewrite with core in *; try discriminate; eauto.
-    apply IHHnf1 in H2 as [? ?]; subst.
-    exfalso; eauto.
-  Qed.
-End CanonicalForms.
-
-Section Progress.
-  Local Hint Constructors stuck : core.
-  Local Hint Constructors step : core.
-  Hint Rewrite nth_error_nil : core.
-
-  Lemma progress_thm : forall e t,
-      [] ⊢ e ∈ t ->
-      stuck e \/ exists e', e -->  e'.
-  Proof.
-    induction e; intros ? Ht; inv Ht;
-      autorewrite with core in *;
-      eauto 3; try discriminate. right.
-    pose proof IHe1 _ H1 as [? | [? ?]]; eauto 3.
-    pose proof IHe2 _ H3 as [? | [? ?]]; eauto 3.
-    pose proof canonical_forms_lambda _ _ _ H H1 as [? ?]; subst; eauto 3.
-  Qed.
-End Progress.
-
-Section Substituion.
-  (** Lemmas inspired by:
-      [http://www.lix.polytechnique.fr/~barras/CoqInCoq/Types.html] *)
-  
-  Local Hint Constructors check : core.
-  Hint Rewrite distr_sub_beta : core.
-  Hint Rewrite shift0 : core.
-  Hint Rewrite Nat.eqb_eq : core.
-  Hint Rewrite Nat.eqb_neq : core.
-  Hint Rewrite nth_error_nil : core.
-
-  Lemma nth_error_length : forall A n l (a : A),
-      nth_error l n = Some a -> n < length l.
-  Proof.
-    induction n; destruct l; intros; simpl in *;
-      try discriminate; try lia.
-    apply IHn in H. lia.
-  Qed.
-
-  Lemma under_prefix : forall e τ Γ Γ',
-      Γ ⊢ e ∈ τ -> (Γ ++ Γ') ⊢ e ∈ τ.
-  Proof.
-    induction e; intros τ g g' H;
-      inv H; simpl in *;
-        autorewrite with core in *;
-        try discriminate; eauto.
+      induction e as [n | t e IHe | e1 IHe1 e2 IHe2];
+      intros G g g' τ Het; inv Het; simpl; eauto.
+    - constructor. destroy_arith.
+      + rewrite Nat.add_comm.
+        rewrite nth_error_app2 in * by lia.
+        replace (length g' + n - length G)
+          with (length g' + (n - length G)) by lia.
+        rewrite nth_error_app_plus. assumption.
+      + rewrite nth_error_app1 in * by lia.
+        assumption.
     - constructor.
-      rewrite nth_error_app1; eauto using nth_error_length.
-    - constructor.
-      replace (t :: g ++ g') with ((t :: g) ++ g') by reflexivity.
-      eauto.
+      replace (S (length G))
+        with (length (t :: G)) by reflexivity.
+      rewrite app_comm_cons. eauto.
   Qed.
 
-  Lemma under_empty : forall e τ Γ,
-      [] ⊢ e ∈ τ -> Γ ⊢ e ∈ τ.
-  Proof.
-    intros. replace Γ with ([] ++ Γ) by reflexivity.
-    auto using under_prefix.
-  Qed.
-
-  Lemma doi : forall a c,
-      a < c -> exists b, a + b = c.
-  Proof.
-    intros ? ? H; induction H.
-    - exists 1. lia.
-    - destruct IHle as [b ?].
-      exists (S b). lia.
-  Qed.
-
-  Lemma nth_error_app_plus : forall A (l l' : list A) n,
-      nth_error (l ++ l') (length l + n) = nth_error l' n.
-  Proof.
-    induction l; intros; simpl in *; eauto.
-  Qed.
-
-  (** The following theorem statements
-      are based of the work of the French.
-      [http://www.lix.polytechnique.fr/~barras/CoqInCoq/Types.html] *)
-  
   Lemma typ_weak_weak : forall e A Γ' Γ T,
       (Γ' ++ Γ) ⊢ e ∈ T ->
       (Γ' ++ A :: Γ) ⊢ shift (length Γ') 1 e ∈ T.
   Proof.
-    induction e; intros ? ? ? ? He;
-      inv He; simpl; eauto; constructor.
-    - destroy_arith.
-      + rewrite nth_error_app1 in * by lia.
-        assumption.
-      + rewrite nth_error_app2 in * by lia.
-        replace (n + 1 - length Γ')
-          with (S (n - length Γ')) by lia.
-        simpl. assumption.
-    - rewrite app_comm_cons.
-      replace (S (length Γ'))
-        with (length (t :: Γ')) by reflexivity.
-      apply IHe. assumption.
+    intros e A G g t Het.
+    replace 1 with (length [A]) by reflexivity.
+    replace (G ++ A :: g)
+      with (G ++ [A] ++ g) by reflexivity.
+    apply typing_shift. assumption.
   Qed.
 
   Lemma thinning : forall e Γ T A,
       Γ ⊢ e ∈ T ->
       (A :: Γ) ⊢ shift 0 1 e ∈ T.
   Proof.
-    intros.
-    replace (A :: Γ)
-      with ([] ++ A :: Γ) by reflexivity.
-    replace 0 with (length (@nil type)) at 1 by reflexivity.
+    intros e g T A Het.
+    replace (A :: g) with ([] ++ A :: g) by reflexivity.
+    replace 0 with (@length type []) at 1 by reflexivity.
     apply typ_weak_weak. assumption.
   Qed.
 
@@ -420,822 +238,189 @@ Section Substituion.
       Γ ⊢ e ∈ T ->
       (Γ' ++ Γ) ⊢ shift 0 (length Γ') e ∈ T.
   Proof.
-    induction Γ' as [| h t IHt]; intros; simpl.
-    - rewrite shift0. assumption.
-    - pose proof thinning as THIN.
-      pose proof simpl_shift as SS.
-      replace (S (length t))
-        with (1 + length t) by reflexivity.
-      rewrite <- simpl_shift with (i := 0) by lia.
-      apply THIN. apply IHt. assumption.
+    intros g' g e t Het.
+    replace (g' ++ g) with ([] ++ g' ++ g) by reflexivity.
+    replace 0 with (@length type nil) by reflexivity.
+    apply typing_shift. assumption.
+  Qed.
+End ShiftLemmas.
+
+Fixpoint sub (n: nat) (es: list expr) (e: expr) : expr :=
+  match e with
+  | !m => if le_lt_dec n m then
+           shift 0 n (nth (m - n) es !(m - n - length es))
+         else !m
+  | λ τ ⇒ e => λ τ ⇒ (sub (S n) es e)
+  | e1 ⋅ e2 => (sub n es e1) ⋅ (sub n es e2)
+  end.
+(**[]*)
+
+Section SubShiftLemmas.
+  Lemma sub_nil : forall e n,
+      sub n [] e = e.
+  Proof.
+    induction e as [m | t e IHe | e1 IHe1 e2 IHe2]; intros; simpl;
+      try (f_equal; eauto; assumption).
+    destroy_arith.
+  Qed.
+    
+  Lemma sub_shift_cancel : forall e n d c ts,
+    c <= n -> length ts + n <= d + c ->
+    sub n ts (shift c d e) = shift c (d - length ts) e.
+  Proof.
+    induction e as [m | t e IHe | e1 IHe1 e2 IHe2]; intros; simpl.
+    - destroy_arith. rewrite nth_overflow by lia.
+      simpl. f_equal. lia.
+    - rewrite IHe by lia. reflexivity.
+    - f_equal; auto.
+  Qed.
+
+  Lemma shift_sub_distr : forall e n d c ts,
+      c <= n -> shift c d (sub n ts e) = sub (d + n) ts (shift c d e).
+  Proof.
+    induction e as [j | t e IHe | e1 IHe1 e2 IHe2]; intros; simpl.
+    - destroy_arith. rewrite shift_add by lia.
+      repeat (f_equal; try lia).
+    - rewrite IHe by lia.
+      do 2 f_equal. lia.
+    - f_equal; auto.
+  Qed.
+
+  Lemma sub_shift_distr :  forall e ts n c d,
+      n <= c ->
+      shift c d (sub n ts e) =
+      sub n (map (shift (c - n) d) ts) (shift (length ts + c) d e).
+  Proof.
+    induction e as [m | t e IHe | e1 IHe1 e2 IHe2];
+      intros; simpl.
+    - destroy_arith; rewrite map_length.
+      + rewrite nth_overflow by lia.
+        replace !(m + d - n - length ts)
+          with (shift (c - n) d !(m - n - length ts)).
+        * rewrite map_nth; simpl. destroy_arith.
+          rewrite nth_overflow by lia; simpl.
+          destroy_arith.
+        * simpl. destroy_arith.
+      + destruct (le_lt_dec (length ts) (m - n)) as [Hmnts | Hmnts].
+        * rewrite nth_overflow by lia.
+          rewrite nth_overflow
+            by (try rewrite map_length; lia).
+          simpl. destroy_arith.
+        * rewrite nth_map with (a := !(m - n - length ts)) by lia.
+          rewrite shift_shift_distr with (c' := 0) by lia.
+          f_equal; try lia.
+    - f_equal. rewrite IHe by lia.
+      f_equal; try lia.
+      f_equal; try lia.
+    - f_equal; auto.
   Qed.
   
-  Lemma typ_sub_weak : forall e e' Γ Γ' τ τ',
-      (Γ ++ τ' :: Γ') ⊢ e ∈ τ ->
-      Γ' ⊢ e' ∈ τ' ->
-      (Γ ++ Γ') ⊢ sub (length Γ) e' e ∈ τ.
+  Lemma sub_sub_distr : forall e n m xs ys,
+      m <= n ->
+      sub n xs (sub m ys e) =
+      sub m (map (sub (n - m) xs) ys) (sub (length ys + n) xs e).
   Proof.
-    induction e; intros ? ? ? ? ? He He';
-      inv He; simpl in *; eauto.
+    induction e as [j | t e IHe | e1 IHe1 e2 IHe2]; intros; simpl.
     - destroy_arith.
-      + constructor.
-        pose proof doi _ _ l as [b Hb]; subst.
-        rewrite <- Nat.add_pred_r by lia.
-        rewrite nth_error_app_plus in H0.
-        rewrite nth_error_app_plus.
-        destruct b; try lia; auto.
-      + replace n with (length Γ + 0) in H0 by lia.
-        rewrite nth_error_app_plus in H0.
-        simpl in *. inv H0. clear Heqs.
-        apply thinning_n. assumption.
-      + constructor.
-        rewrite nth_error_app1 in * by lia; auto.
-    - constructor.
-      replace (t :: Γ ++ Γ')
-        with ((t :: Γ) ++ Γ') by reflexivity.
-      replace (S (length Γ))
-        with (length (t :: Γ)) by reflexivity.
-      apply IHe with τ'; simpl; auto.
+      + rewrite nth_overflow by lia; simpl. destroy_arith.
+        rewrite sub_shift_cancel
+          by (try rewrite map_length; lia).
+        rewrite map_length. do 3 (f_equal; try lia).
+      + rewrite map_length.
+        destruct (le_lt_dec (length ys) (j - m)) as [Hjmys | Hjmys].
+        * rewrite nth_overflow by lia.
+          rewrite nth_overflow
+            by (try rewrite map_length; lia).
+          simpl. destroy_arith.
+        * rewrite nth_map with (a := !(j - m - length ys)) by lia.
+          rewrite shift_sub_distr by lia.
+          f_equal; lia.
+    - f_equal. rewrite IHe by lia.
+      f_equal; try lia.
+      f_equal; try lia.
+    - f_equal; auto.
   Qed.
 
-  Lemma substitution_lemma : forall Γ τ τ' e e',
-    (τ' :: Γ) ⊢ e ∈ τ -> Γ ⊢ e' ∈ τ' -> Γ ⊢ beta_reduce e e' ∈ τ.
+  Lemma sub_append : forall e xs ys n,
+      sub n (xs ++ ys) e = sub n xs (sub (length xs + n) ys e).
   Proof.
-    intros ? ? ? ? ? He He'; unfold beta_reduce.
-    replace Γ with ([] ++ Γ) by reflexivity.
-    eapply typ_sub_weak; eauto.
+    induction e as [m | t e IHe | e1 IHe1 e2 IHe2];
+      intros; simpl.
+    - destroy_arith.
+      + rewrite app_nth2 by lia.
+        rewrite sub_shift_cancel by lia.
+        rewrite app_length.
+        repeat (f_equal; try lia).
+      + rewrite app_nth1 by lia.
+        rewrite app_length.
+        repeat (f_equal; try lia).
+    - f_equal. rewrite IHe by lia.
+      repeat (f_equal; try lia).
+    - f_equal; auto.
   Qed.
-End Substituion.
 
-Section Preservation.
-  Local Hint Constructors check : core.
+  Local Hint Constructors typing : core.
 
-  Theorem preservation : forall e e' Γ τ,
-    e -->  e' -> Γ ⊢ e ∈ τ -> Γ ⊢ e' ∈ τ.
+  Lemma typing_sub : forall e G ts g T es,
+      Forall2 (typing g) es ts ->
+      (G ++ ts ++ g) ⊢ e ∈ T ->
+      (G ++ g) ⊢ sub (length G) es e ∈ T.
   Proof.
-    intros ? ? g t He; generalize dependent t;
-      generalize dependent g;
-      induction He; intros ? ? Ht; inv Ht; eauto.
-    - inv H2. eapply substitution_lemma; eauto.
+    intro e;
+      induction e as [n | t e IHe | e1 IHe1 e2 IHe2];
+      intros G ts g T es HF2 Het; inv Het; simpl; eauto.
+    - assert (Hlen : length es = length ts)
+        by eauto using Forall2_length.
+      destroy_arith.
+      + apply thinning_n.
+        destruct (le_lt_dec (length es) (n - length G))
+          as [Hesng | Hesng].
+        * rewrite nth_overflow by lia.
+          constructor. rewrite Hlen.
+          repeat rewrite nth_error_app2 in H0 by lia.
+          assumption.
+        * rewrite nth_error_app2 in H0 by lia.
+          rewrite nth_error_app1 in H0 by lia.
+          apply length_nth_error in Hesng as [e Hnth].
+          erewrite nth_error_nth by eauto.
+          eapply Forall2_nth_error; eauto.
+      + rewrite nth_error_app1 in H0 by lia.
+        constructor. rewrite nth_error_app1 by lia.
+        assumption.
+    - replace (S (length G))
+        with (length (t :: G)) by reflexivity.
+      constructor. rewrite app_comm_cons. eauto.
   Qed.
-End Preservation.
+End SubShiftLemmas.
 
-Notation "e1 '-->*' e2" := (refl_trans_closure step e1 e2) (at level 40).
-
-Section MultiStep.
-  Local Hint Constructors step : core.
-  Local Hint Constructors refl_trans_closure : core.
-  
-  Lemma multi_step_app_l : forall e1 e1' e2,
-    e1 -->* e1' -> e1 ⋅ e2 -->*  e1' ⋅ e2.
-  Proof.
-    intros ? ? e2 Hms;
-      generalize dependent e2;
-      induction Hms; eauto.
-  Qed.
-
-  Lemma multi_step_app_r : forall e1 e2 e2',
-      stuck e1 -> e2 -->* e2' -> e1 ⋅ e2 -->*  e1 ⋅ e2'.
-  Proof.
-    intros e1 ? ? ? Hms;
-      generalize dependent e1;
-      induction Hms; eauto.
-  Qed.
-End MultiStep.
-
-(** Does a program halt? *)
-Definition halts (e : expr) : Prop :=
-  exists e', e -->* e' /\ forall e'', ~ e' -->  e''.
+(** Beta-reduction [(λx.e1) e2 -> e1{e2/x}]. *)
+Definition beta_reduce (e1 e2 : expr) : expr := sub 0 [e2] e1.
 (**[]*)
 
-Section NH.
-  Local Hint Constructors refl_trans_closure : core.
-  Local Hint Resolve stuck_step : core.
-  
-  Lemma stuck_halts : forall e, stuck e -> halts e.
-  Proof. intros ? ?; unfold halts; eauto 4. Qed.
-End NH.
-
-Inductive closed : nat -> expr -> Prop :=
-| closed_var k n :
-    n < k ->
-    closed k !n
-| closed_lam k t e :
-    closed (S k) e ->
-    closed k (λ t ⇒ e)
-| closed_app k e1 e2 :
-    closed k e1 ->
-    closed k e2 ->
-    closed k (e1 ⋅ e2).
-(**[]*)
-
-(** This property is necessary
-    to prove some properties of [R]. *)
-Lemma type_closed : forall Γ e t,
-    Γ ⊢ e ∈ t -> closed (length Γ) e.
+Lemma typing_beta_reduce : forall g e E t T,
+    g ⊢ e ∈ t ->
+    (t :: g) ⊢ E ∈ T ->
+    g ⊢ (beta_reduce E e) ∈ T.
 Proof.
-  intros ? ? ? H; induction H;
-    constructor; simpl in *; auto.
-  eapply nth_error_length; eauto.
-Qed.
-
-Lemma empty_context_closed : forall e t,
-    [] ⊢ e ∈ t -> closed 0 e.
-Proof.
-  intros.
+  intros g e E t T He HE. unfold beta_reduce.
+  replace g with ([] ++ g) by reflexivity.
   replace 0 with (@length type []) by reflexivity.
-  eapply type_closed; eauto 1.
+  eapply typing_sub; eauto.
 Qed.
-
-Section FrenchLemmas.
-  Local Hint Constructors stuck : core.
-  Local Hint Constructors is_lam : core.
-
-  Lemma is_lam_shift : forall e k i,
-      is_lam (shift k i e) -> is_lam e.
-  Proof.
-    intros [] ? ? H; inv H; auto.
-  Qed.
-
-  Local Hint Resolve is_lam_shift : core.
-
-  Lemma stuck_shift : forall e k i,
-      stuck e -> stuck (shift k i e).
-  Proof.
-    intros ? k i Hstk;
-      generalize dependent i;
-      generalize dependent k;
-      induction Hstk; simpl;
-        destroy_arith; eauto.
-  Qed.
-
-  Local Hint Resolve stuck_shift : core.
   
-  Lemma stuck_sub : forall e,
-      stuck e -> forall i esub, stuck esub -> stuck (sub i esub e).
-  Proof.
-    intros ? Hv; induction Hv; intros; simpl; auto.
-    - destroy_arith; auto 1.
-    - constructor; eauto.
-  Abort.
-  
-  Local Hint Constructors step : core.
-  (* Local Hint Resolve stuck_sub : core. *)
-  
-  Lemma sub_step : forall e e' es i,
-      stuck es ->
-      e -->  e' ->
-      sub i es e -->  sub i es e'.
-  Proof.
-    intros ? ? ? es i H.
-      generalize dependent es;
-      generalize dependent i.
-      induction H; intros; simpl; eauto.
-      rewrite distr_sub_beta; auto.
-  Abort.
-  
-  Lemma beta_reduce_step : forall e1 e1' e2,
-      stuck e2 ->
-      e1 -->  e1' ->
-      beta_reduce e1 e2 -->  beta_reduce e1' e2.
-  Proof.
-    unfold beta_reduce; intros.
-    Fail apply sub_step; assumption.
-  Abort.
+Reserved Notation "e1 '-->' e2" (at level 40).
 
-  Hint Constructors closed : core.
-  
-  Lemma closed_closed : forall e m n,
-      m < n -> closed m e -> closed n e.
-  Proof.
-    induction e; intros ? ? ? Hm; inv Hm; eauto.
-    - constructor. lia.
-    - constructor.
-      apply IHe with (S m); auto 1; lia.
-  Qed.
-
-  Lemma shift_closed : forall k e,
-      closed k e -> forall c i, closed (k + i) (shift c i e).
-  Proof.
-    intros k e Hc; induction Hc;
-      intros c i; simpl; eauto.
-    constructor. destroy_arith.
-  Qed.
-End FrenchLemmas.
-
-Section StepEXM.
-  Local Hint Constructors step : core.
-  Local Hint Constructors stuck : core.
-  Local Hint Constructors is_lam : core.
-
-  Lemma nstuck_step_exists : forall e,
-      ~ stuck e -> exists e', e -->  e'.
-  Proof.
-    intro e;
-      induction e as
-        [ n
-        | t e IHe
-        | e1 IHe1 e2 IHe2 ]; intros Hstk;
-        try (exfalso; auto; contradiction).
-    destruct (stuck_exm e1) as [He1 | He1].
-    - destruct (stuck_exm e2) as [He2 | He2].
-      + destruct (is_lam_exm e1) as [Hl1 | Hl1].
-        * inv Hl1; eauto.
-        * exfalso; auto.
-      + apply IHe2 in He2 as [? ?]; eauto.
-    - apply IHe1 in He1 as [? ?]; eauto.
-  Qed.
-
-  Local Hint Resolve nstuck_step_exists : core.
-
-  Lemma nstep_stuck : forall e,
-      (forall e', ~ e -->  e') -> stuck e.
-  Proof.
-    intros e H.
-    destruct (stuck_exm e) as [Hstk | Hstk]; auto.
-    apply nstuck_step_exists in Hstk as [? Hstep].
-    apply H in Hstep. contradiction.
-  Qed.
-        
-  Lemma step_exm : forall e,
-      (exists e', e -->  e') \/ forall e', ~ e -->  e'.
-  Proof.
-    intro e;
-      pose proof stuck_exm e as [H | H];
-      intuition. right; intros e'.
-    eapply stuck_step in H; eauto.
-  Qed.
-End StepEXM.
-
-Section Forall2Context.
-  Context {U V : Type}.
-
-  Section Defs.
-    Variable R : list U -> V -> U -> Prop.
-    Variable ctx : list U.
-
-    Inductive AllCtx2 : list V -> list U -> Prop :=
-    | AllCtx2_nil :
-        AllCtx2 [] []
-    | AllCtx2_cons u us v vs :
-        R (us ++ ctx) v u ->
-        AllCtx2 vs us ->
-        AllCtx2 (v :: vs) (u :: us).
-    (**[]*)
-
-    Lemma AllCtx2_length : forall vs us,
-        AllCtx2 vs us -> length vs = length us.
-    Proof.
-      intros vs us H; induction H; simpl; auto.
-    Qed.
-  End Defs.
-
-  Local Hint Constructors AllCtx2 : core.
-
-  Lemma AllCtx2_sanity : forall (R : V -> U -> Prop) ctx vs us,
-      AllCtx2 (fun _ => R) ctx vs us <-> Forall2 R vs us.
-  Proof.
-    intros ? ? ? ?; split; intros H;
-      induction H; auto.
-  Qed.
-
-  Lemma AllCtx2_impl : forall (R W : list U -> V -> U -> Prop) ctx vs us,
-      (forall ctx v u, R ctx v u -> W ctx v u) ->
-      AllCtx2 R ctx vs us -> AllCtx2 W ctx vs us.
-  Proof.
-    intros R W ctx vs us HRW HR; induction HR; auto.
-  Qed.
-End Forall2Context.
-
-Lemma Forall2_length : forall A B (R : A -> B -> Prop) a b,
-    Forall2 R a b -> length a = length b.
-Proof.
-  intros A B R a b H; induction H; simpl; auto.
-Qed.
-
-Lemma Forall2_impl : forall A B (P Q : A -> B -> Prop) a b,
-    (forall a b, P a b -> Q a b) ->
-    Forall2 P a b -> Forall2 Q a b.
-Proof.
-  intros A B P Q a b H HP;
-    induction HP; auto.
-Qed.
-
-Lemma rev_nil : forall A (l : list A), rev l = [] -> l = [].
-Proof.
-  intros A l;
-    induction l as [| h t IHt] using rev_ind;
-    intros H; trivial.
-  rewrite rev_unit in H. discriminate.
-Qed.
-
-Module JapaneseNorm.
-  Lemma sub_closed : forall k e,
-    closed k e -> forall n v, sub (k + n) v e = e.
-  Proof.
-    intros k e HC; induction HC;
-      intros; simpl; destroy_arith;
-        f_equal; eauto.
-  Qed.
-
-  Inductive all_closed (k : nat) : list expr -> Prop :=
-  | all_closed_nil :
-      all_closed k []
-  | all_closed_cons v vs :
-      closed (length vs + k) v ->
-      all_closed k vs ->
-      all_closed k (v :: vs).
-  (**[]*)
-    
-  Section FoldSub.
-    Lemma sub_fold_sub : forall k e v vs,
-      sub k v (fold_left (fun e v => sub k v e) vs e) =
-      fold_left (fun e v => sub k v e) (vs ++ [v]) e.
-    Proof.
-      intros k e v vs.
-      rewrite fold_left_app; simpl.
-      reflexivity.
-    Qed.
-
-    Lemma distr_fold_sub : forall vs M N n p,
-        fold_left (fun e v => sub (p + n) v e) vs (sub p N M) =
-        sub p (fold_left (fun e v => sub n v e) vs N)
-            (fold_left (fun e v => sub (S (p + n)) v e) vs M).
-    Proof.
-      intro vs; induction vs as [| v vs IHvs];
-        intros M N n p; simpl; trivial.
-      rewrite <- IHvs. rewrite distr_sub. reflexivity.
-    Qed.
-
-    Lemma distr_fold_br : forall vs M N n,
-        fold_left (fun e v => sub n v e) vs (beta_reduce M N) =
-        beta_reduce
-          (fold_left (fun e v => sub (S n) v e) vs M)
-          (fold_left (fun e v => sub n v e) vs N).
-    Proof.
-      intros vs M N n; unfold beta_reduce.
-      replace n with (0 + n) by reflexivity.
-      rewrite distr_fold_sub. reflexivity.
-    Qed.
-    
-    Lemma fold_sub_closed_l : forall vs e k n,
-        closed k e ->
-        fold_left (fun e v => sub (k + n) v e) vs e = e.
-    Proof.
-      intro vs; induction vs as [| v vs IHvs];
-        intros; simpl; trivial.
-      rewrite sub_closed by assumption.
-      firstorder.
-    Qed.
-
-    Local Hint Resolve sub_closed : core.
-
-    Lemma fold_sub_closed_r : forall vs e k n,
-        closed k e ->
-        fold_right (sub (k + n)) e vs = e.
-    Proof.
-      intro vs; induction vs as [| v vs IHvs];
-        intros; simpl; trivial.
-      rewrite IHvs by assumption; auto.
-    Qed.
-
-    Local Hint Resolve typ_sub_weak : core.
-    
-    Lemma fold_typ_sub_weak_l : forall vs ts g,
-        AllCtx2 check g vs ts ->
-        forall G e t,
-          (G ++ ts ++ g) ⊢ e ∈ t ->
-          (G ++ g) ⊢ fold_left (fun e v => sub (length G) v e) vs e ∈ t.
-    Proof.
-      intros vs ts g Hctx;
-        induction Hctx; intros G e t Het;
-          simpl in *; eauto.
-    Qed.
-
-    Lemma fold_typ_sub_weak_r : forall vs ts g,
-        AllCtx2 check g vs ts ->
-        forall G e t,
-          (G ++ rev ts ++ g) ⊢ e ∈ t ->
-          (G ++ g) ⊢ fold_right (sub (length G)) e vs ∈ t.
-    Proof.
-      intros vs ts g Hctx;
-        induction Hctx; intros G e t Het;
-          simpl in *; trivial.
-      apply typ_sub_weak with u.
-    Abort.
-
-    Lemma fold_sub_lambda_l : forall vs e t n,
-        fold_left (fun e v => sub n v e) vs (λ t ⇒ e) =
-        λ t ⇒ (fold_left (fun e v => sub (S n) v e) vs e).
-    Proof.
-      intro vs; induction vs as [| v vs IHvs];
-        intros e t n; simpl; trivial.
-    Qed.
-
-    Lemma fold_sub_app_l : forall vs e1 e2 n,
-        fold_left (fun e v => sub n v e) vs (e1 ⋅ e2) =
-        (fold_left (fun e v => sub n v e) vs e1) ⋅ (fold_left (fun e v => sub n v e) vs e2).
-    Proof.
-      intro vs; induction vs as [| v vs IHvs];
-        intros e t n; simpl; trivial.
-    Qed.        
-  End FoldSub.
-
-  Fixpoint msub (n : nat) (vs : list expr) (e : expr) : expr :=
-    match vs with
-    | [] => e
-    | v :: vs => msub n vs (sub (n + length vs) v e)
-    end.
-  (**[]*)
-
-  Section MSub.
-    Lemma msub_closed : forall vs e k,
-      closed k e ->
-      msub k vs e = e.
-    Proof.
-      intro vs;
-        induction vs as [| v vs IHvs];
-        intros e k Hek; simpl; trivial.
-      rewrite sub_closed by assumption; auto.
-    Qed.
-
-    Local Hint Resolve sub_closed : core.
-
-    Lemma typ_msub_weak : forall vs ts g,
-        Forall2 (check g) vs ts ->
-        forall G e t,
-          (G ++ rev ts ++ g) ⊢ e ∈ t ->
-          (G ++ g) ⊢ msub (length G) vs e ∈ t.
-    Proof.
-      intro vs;
-        induction vs as [| v vs IHvs];
-        intros [| t ts] g HF2 G e τ Het;
-        inv HF2; simpl in *; trivial.
-      apply IHvs with (ts := ts); auto.
-      assert (Hlen : length vs = length ts) by eauto using Forall2_length.
-      rewrite Hlen. rewrite <- (rev_length ts).
-      rewrite <- app_length. rewrite app_assoc.
-      eapply typ_sub_weak; eauto.
-      rewrite <- app_assoc in Het; simpl in Het.
-      rewrite app_assoc in Het. assumption.
-    Qed.
-    
-    Lemma msub_lambda : forall vs e t n,
-        msub n vs (λ t ⇒ e) = λ t ⇒ (msub (S n) vs e).
-    Proof.
-      intro vs; induction vs as [| v vs IHvs];
-        intros e t n; simpl; trivial.
-    Qed.
-
-    Lemma msub_app : forall vs e1 e2 n,
-        msub n vs (e1 ⋅ e2) = (msub n vs e1) ⋅ (msub n vs e2).
-    Proof.
-      intro vs; induction vs as [| v vs IHvs];
-        intros e1 e2 n; simpl; trivial.
-    Qed.
-
-    Lemma msub_single : forall n v e,
-        msub n [v] e = sub n v e.
-    Proof.
-      intros n v e; simpl.
-      rewrite Nat.add_comm. reflexivity.
-    Qed.
-
-    Lemma msub_append : forall vs1 vs2 e n,
-        msub n (vs1 ++ vs2) e = msub n vs2 (msub (n + length vs2) vs1 e).
-    Proof.
-      intro vs1; induction vs1 as [| v1 vs1 IHvs1];
-        intros vs2 e n; simpl; trivial.
-      rewrite IHvs1. rewrite app_length.
-      rewrite (Nat.add_comm (length vs1) (length vs2)).
-      rewrite Nat.add_assoc. reflexivity.
-    Qed.
-
-    Lemma msub_sub : forall vs n e v,
-        sub n v (msub (S n) vs e) = msub n (vs ++ [v]) e.
-    Proof.
-      intros vs n e v.
-      rewrite <- msub_single.
-      rewrite msub_append; simpl.
-      repeat f_equal; lia.
-    Qed.
-
-    Lemma sub_msub : forall vs n k e v,
-        sub n v (msub (n + k) vs e) = msub n (vs ++ [v]) e.
-    Proof.
-      intro vs; induction vs as [| v vs IHvs];
-        intros n k e e'; simpl.
-      - f_equal; lia.
-      - rewrite IHvs.
-    Abort.
-
-    Lemma msub_var : forall vs v k n,
-        Forall (closed k) vs ->
-        nth_error vs n = Some v ->
-        msub k vs !n = v.
-    Proof.
-      intro vs; induction vs as [| v vs IHvs];
-        intros e k n Hvs Hnth; inv Hvs; simpl.
-      - rewrite nth_error_nil in Hnth; discriminate.
-      - destruct n as [| n]; simpl in *; destroy_arith.
-        + inv Hnth. rewrite e0.
-          rewrite shift0. apply msub_closed; auto.
-        + inv Hnth. rewrite IHvs with (v := e); auto.
-          admit.
-        + rewrite e0. admit.
-        + rewrite IHvs with (v := e); auto.
-    Abort.
-  End MSub.
-  
-  (** Strongly normalizing. *)
-  Inductive SN (e : expr) : Prop :=
-  | SN_intro :
-      (forall e', e -->  e' -> SN e') -> SN e.
-  (**[]*)
-
-  Section SNProp.
-    Local Hint Constructors refl_trans_closure : core.
-    
-    Lemma SN_halts : forall e, SN e -> halts e.
-    Proof.
-      unfold halts; intros e H; induction H.
-      destruct (step_exm e) as [[e' He] | He]; eauto 3.
-      apply H0 in He as He'.
-      destruct He' as [e'' [He' He'']]; eauto 4.
-    Qed.
-
-    Local Hint Constructors step : core.
-
-    Lemma step_SN : forall e e',
-        e -->  e' -> SN e -> SN e'.
-    Proof.
-      intros ? ? ? HSN; inv HSN; eauto.
-    Qed.
-
-    Lemma unstep_SN : forall e e',
-        e -->  e' -> SN e' -> SN e.
-    Proof.
-      intros e e' Hs HSN; constructor.
-      intros e'' Hs';
-        pose proof step_deterministic _ _ _ Hs Hs';
-        subst; auto.
-    Qed.
-
-    Local Hint Constructors is_lam : core.
-    Local Hint Constructors stuck : core.
-    Local Hint Resolve step_nstuck : core.
-
-    Lemma stuck_SN : forall v, stuck v -> SN v.
-    Proof.
-      intros ? Hv; induction Hv;
-        constructor; intros ? Hstep; inv Hstep;
-          try (exfalso; eauto; contradiction).
-      - apply step_nstuck in H4. contradiction.
-      - apply step_nstuck in H3. contradiction.
-    Qed.
-
-    Local Hint Resolve stuck_SN : core.
-
-    Lemma SN_var : forall n, SN !n.
-    Proof. intuition. Qed.
-
-    Lemma SN_lambda : forall t e, SN (λ t ⇒ e).
-    Proof. intuition. Qed.
-
-    Local Hint Resolve nstep_stuck : core.
-    
-    Lemma SN_exists_stuck : forall e,
-        SN e -> exists v, stuck v /\ e -->* v.
-    Proof.
-      intros e Hsn.
-      apply SN_halts in Hsn as [e' [Hms He']]; eauto.
-    Qed.
-  End SNProp.
-
-  (** The logical relation. *)
-  Fixpoint R (g : list type) (e : expr) (t : type) : Prop :=
-    SN e /\ g ⊢ e ∈ t /\
-    match t with
-    | ⊥ => True
-    | t → t' => forall e2, R g e2 t -> R g (e ⋅ e2) t'
-    end.
-  (**[]*)
-
-  Section RProp.
-    Local Hint Resolve step_SN : core.
-    Local Hint Constructors step : core.
-
-    Lemma R_types : forall g e t, R g e t -> g ⊢ e ∈ t.
-    Proof.
-      intros ? ? []; simpl; firstorder.
-    Qed.
-
-    Lemma R_SN : forall g e t, R g e t -> SN e.
-    Proof.
-      intros ? ? []; simpl; firstorder.
-    Qed.
-
-    Local Hint Resolve preservation : core.
-    
-    Lemma step_R : forall t g e e',
-      e -->  e' -> R g e t -> R g e' t.
-    Proof.
-      intro t; induction t; intros;
-        simpl in *; intuition; eauto.
-    Qed.
-    
-    Local Hint Resolve unstep_SN : core.
-    Local Hint Resolve R_types : core.
-    Local Hint Resolve R_SN : core.
-    Local Hint Constructors SN : core.
-    Local Hint Constructors check : core.
-
-    Lemma unstep_R : forall t g e e',
-        e -->  e' -> g ⊢ e ∈ t -> R g e' t -> R g e t.
-    Proof.
-      intro t; induction t; intros;
-        simpl in *; intuition; eauto 6.
-    Qed.
-    
-    Local Hint Resolve step_R : core.
-    Local Hint Resolve unstep_R : core.
-    Local Hint Constructors stuck : core.
-    Local Hint Resolve stuck_SN : core.
-
-    Lemma multi_step_R : forall e e' g t,
-        e -->* e' -> R g e t -> R g e' t.
-    Proof.
-      intros ? ? ? ? Hms;
-        induction Hms; simpl; eauto.
-    Qed.
-
-    Lemma multi_unstep_R : forall e e' g t,
-        e -->* e' -> g ⊢ e ∈ t -> R g e' t -> R g e t.
-    Proof.
-      intros ? ? ? ? Hms;
-        induction Hms; eauto.
-    Qed.
-
-    Local Hint Resolve multi_step_R : core.
-    Local Hint Resolve multi_unstep_R : core.
-    Local Hint Resolve trans_closure_r : core.
-    Local Hint Resolve multi_step_app_r : core.
-
-    Lemma abs_R_sub : forall g e t t',
-        g ⊢ λ t ⇒ e ∈ t → t' ->
-        (forall G v, R (G ++ g) v t -> R (G ++ g) (sub (length G) v e) t') ->
-        R g (λ t ⇒ e) (t → t').
-    Proof.
-      intros g e t t' Het HR; simpl; intuition.
-      assert (Hsn : SN e2) by eauto.
-      apply SN_exists_stuck in Hsn as [v [Hvstk Hvms]].
-      apply multi_unstep_R with (e' := beta_reduce e v); eauto.
-      unfold beta_reduce.
-      replace 0 with (@length type []) by reflexivity.
-      pose proof HR []; simpl in *; eauto.
-    Qed.
-
-    Lemma abs_R : forall g e t t',
-        g ⊢ λ t ⇒ e ∈ t → t' ->
-        (forall v, stuck v -> R g v t -> R g (beta_reduce e v) t') ->
-        R g (λ t ⇒ e) (t → t').
-    Proof.
-      intros g e t t' Het HR; simpl; intuition.
-      assert (Hsn : SN e2) by eauto.
-      apply SN_exists_stuck in Hsn as [v [Hvstk Hvms]].
-      apply multi_unstep_R with (e' := beta_reduce e v); eauto.
-    Qed.
-
-    Local Hint Resolve SN_lambda : core.
-    Local Hint Resolve SN_var : core.
-    Local Hint Resolve typ_msub_weak : core.
-    Local Hint Resolve fold_typ_sub_weak_l : core.
-    Local Hint Resolve AllCtx2_impl : core.
-
-    (*Definition br_first*)
-
-    Lemma R_fold_br : forall g ts e t vs,
-        AllCtx2 R g vs ts ->
-        (ts ++ g) ⊢ e ∈ t ->
-        R g (fold_left beta_reduce vs e) t.
-    Proof.
-      intros g ts e t vs ? Het.
-      remember (ts ++ g) as Γ eqn:Heqg.
-      generalize dependent g; generalize dependent ts; generalize dependent vs.
-      induction Het; intros vs ts g Hctx Heqg; subst.
-      - generalize dependent n;
-          generalize dependent τ.
-        induction Hctx; intros t n Hnth; simpl in *.
-        + generalize dependent n;
-            generalize dependent t.
-          induction g as [| tg g IHg];
-            intros t n Hnth; simpl.
-          * rewrite nth_error_nil in Hnth.
-            discriminate.
-          * destruct n as [| n]; simpl in *.
-            ** inv Hnth. generalize dependent g.
-               induction t as [| t1 IHt1 t2 IHt2];
-                 intros g IH; simpl; intuition. admit.
-            ** admit.
-        + admit.
-      - unfold beta_reduce.
-        rewrite fold_sub_lambda_l. apply abs_R.
-        + constructor.
-          replace (τ :: g) with ([τ] ++ g) by reflexivity.
-          replace 1 with (length [τ]) by reflexivity. eauto.
-        + intros v Hstk HR. admit.
-      - assert (doi: ts ++ g = ts ++ g) by reflexivity.
-        pose proof IHHet1 _ _ _ Hctx doi as IH1.
-        pose proof IHHet2 _ _ _ Hctx doi as IH2.
-        unfold beta_reduce in *.
-        rewrite fold_sub_app_l. simpl in IH1.
-        intuition.
-    Admitted.
-
-    Lemma R_fold_sub : forall G ts g e t vs,
-        AllCtx2 R g vs ts ->
-        (G ++ ts ++ g) ⊢ e ∈ t ->
-        R (G ++ g) (fold_left (fun e v => sub (length G) v e) vs e) t.
-    Proof.
-      intros G ts g e t vs ? Het. generalize dependent vs.
-      remember (G ++ ts ++ g) as Γ eqn:HeqG.
-      generalize dependent g; generalize dependent ts; generalize dependent G.
-      induction Het; intros G ts g Heqg vs Hac; subst.
-      - admit.
-      - simpl; intuition.
-        + rewrite fold_sub_lambda_l. eauto.
-        + rewrite fold_sub_lambda_l.
-          constructor.
-          replace (S (length G))
-            with (length (τ :: G)) by reflexivity.
-          rewrite app_comm_cons. eauto.
-        + assert (Hsn : SN e2) by eauto.
-          apply SN_exists_stuck in Hsn as [v [Hv He2]].
-          apply multi_unstep_R
-            with (e' :=
-                    beta_reduce
-                      (fold_left
-                         (fun e v => sub (S (length G)) v e) vs e) v).
-          * rewrite fold_sub_lambda_l; eauto.
-          * constructor 3 with τ; eauto.
-          * assert (doi: τ :: G ++ ts ++ g = τ :: G ++ ts ++ g) by trivial.
-            pose proof IHHet (τ :: G) ts g doi vs Hac as IH; clear IHHet.
-            simpl in *.
-            Check substitution_lemma.
-            (** Maybe "substitution_lemma" for R? *) admit.
-      - rewrite fold_sub_app_l.
-        assert (doi: G ++ ts ++ g = G ++ ts ++ g) by trivial.
-        pose proof IHHet1 G ts g doi vs Hac.
-        pose proof IHHet2 G ts g doi vs Hac.
-        simpl in *; intuition.
-    Admitted.
-
-    Local Hint Resolve Forall2_impl : core.
-    
-    Lemma R_msub : forall G ts g e t vs,
-        Forall2 (R g) vs ts ->
-        (G ++ rev ts ++ g) ⊢ e ∈ t ->
-        R (G ++ g) (msub (length G) vs e) t.
-    Proof.
-      intros G ts g e t vs ? Het.
-      generalize dependent vs.
-      remember (G ++ rev ts ++ g) as ctx eqn:Hctxeq.
-      generalize dependent g;
-        generalize dependent ts;
-        generalize dependent G.
-      induction Het; intros G ts g Heqctx vs HF2; subst.
-      - admit.
-      - rewrite msub_lambda.
-        replace (S (length G))
-          with (length (τ :: G)) by reflexivity.
-        unfold R; fold R; intuition.
-        + constructor.
-          rewrite app_comm_cons; eauto.
-        + assert (Hsn: SN e2) by eauto.
-          apply SN_exists_stuck in Hsn as [v [Hstk Hms]].
-          apply multi_unstep_R with
-              (e' := beta_reduce (msub (length (τ :: G)) vs e) v); eauto.
-          * constructor 3 with τ; eauto.
-            constructor.
-            rewrite app_comm_cons; eauto.
-          * unfold beta_reduce. admit.
-      - rewrite msub_app.
-        assert (Hdumb : G ++ rev ts ++ g = G ++ rev ts ++ g)
-          by trivial.
-        pose proof IHHet1 _ _ _ Hdumb _ HF2
-          as [HSN [Hchk HR]]; clear IHHet1.
-        pose proof IHHet2 _ _ _ Hdumb _ HF2 as IH2; clear IHHet2.
-        eauto.
-    Admitted.
-
-    Lemma reduce_lemma : forall e t g ts vs,
-        Forall2 (R g) vs ts ->
-        (ts ++ g) ⊢ e ∈ t ->
-        R g (fold_left beta_reduce vs e) t.
-    Proof.
-      intro e;
-        induction e as [n | t e IHe | e1 IHe1 e2 IHe2];
-        intros τ g ts vs HF2 Het; inv Het; simpl.
-    Abort.
-  End RProp.
-End JapaneseNorm.
+(** Beta-reduction. *)
+Inductive bred : expr -> expr -> Prop :=
+| bred_bred t e1 e2 :
+    (λ t ⇒ e1) ⋅ e2 -->  beta_reduce e1 e2
+| bred_abs t e e' :
+    e -->  e' ->
+    λ t ⇒ e -->  λ t ⇒ e'
+| bred_app_l el el' er :
+    el -->  el' ->
+    el ⋅ er -->  el' ⋅ er
+| bred_app_r el er er' :
+    er -->  er' ->
+    el ⋅ er -->  el ⋅ er'
+where "e1 '-->' e2" := (bred e1 e2).
